sitpn2hvhdl/Soundness.v
@@ -4,9 +4,11 @@ Require Import GlobalTypes.
 
 (* SITPN Libraries *)
 
-Require Import SitpnTypes.
-Require Import Sitpn.
+Require Import dp.SitpnTypes.
+Require Import dp.Sitpn.
 Require Import dp.SitpnSemantics.
+Require Import dp.Fired.
+
 
 (* H-VHDL Libraries *)
 
@@ -14,10 +16,13 @@ Require Import HVhdlTypes.
 Require Import Environment.
 Require Import SemanticalDomains.
 Require Import Simulation.
+Require Import CombinationalEvaluation.
+Require Import SynchronousEvaluation.
 Require Import DesignElaboration.
 Require Import AbstractSyntax.
 Require Import HilecopDesignStore.
 Require Import Initialization.
+Require Import Stabilize.
 
 (* SITPN to H-VHDL Libraries *)
 
@@ -44,7 +49,8 @@ Definition EnvEq sitpn (Ec : nat -> C sitpn -> bool) (Ep : nat -> Clk -> IdMap v
     a H-VHDL design state.
  *)
 
-Definition SimState {sitpn} (s : SitpnState sitpn) (dstate : DState) : Prop := False.
+Definition SimState {sitpn} (s : SitpnState sitpn) (σ : DState) : Prop := False.
+Local Notation "s '∼' σ" := (SimState s σ) (at level 50).
 
 (** ** Simulation Lemma *)
 
@@ -109,7 +115,7 @@ Admitted.
 (** ** Semantic Preservation Theorem *)
 
 Theorem sitpn2vhdl_sound :
-  forall sitpn Ec tau s' d Mg Ep dstate' mm,
+  forall sitpn Ec τ s' d Mg Ep σ' mm,
 
     (* sitpn translates into d. *)
     sitpn_to_hvhdl sitpn mm = Success d ->
@@ -117,18 +123,18 @@ Theorem sitpn2vhdl_sound :
     (* Environments are similar. *)
     EnvEq sitpn Ec Ep ->      
 
-    (* sitpn is in state s after tau execution cycles. *)
-    SitpnExecute Ec (s0 sitpn) tau s' ->
+    (* sitpn is in state s after \tau execution cycles. *)
+    SitpnExecute Ec (s0 sitpn) τ s' ->
     
-    (* d is in state dstate after tau execution cycles. *)
-    simwf hdstore Mg Ep tau d dstate' ->
+    (* d is in state dstate after \tau execution cycles. *)
+    simwf hdstore Mg Ep τ d σ' ->
 
     (* ** Conclusion: final states are equal. ** *)
-    SimState s' dstate'.
+    SimState s' σ'.
 Proof.
   inversion_clear 4.
 
-  match goal with
+  lazymatch goal with
   | [
     Htransl: sitpn_to_hvhdl _ _ = _,
     Henveq: EnvEq _ _ _,
@@ -138,10 +144,45 @@ Proof.
     Hsimloop: simloop _ _ _ _ _ _
     |- _ ] =>
     specialize (init_states_sim sitpn mm d Mg ed dstatee dstate0 Htransl Helab Hinit) as Hinit_eq; 
-      apply (simulation_lemma sitpn Ec (s0 sitpn) s' tau Hsitpnexec 
-                              Mg d Ep dstate0 dstate' ed dstatee mm
+      apply (simulation_lemma sitpn Ec (s0 sitpn) s' τ Hsitpnexec 
+                              Mg d Ep dstate0 σ' ed dstatee mm
                               Htransl Henveq Helab Hinit_eq Hsimloop)
   end.
 
 Qed.
-  
+
+Lemma falling_edge_compute_fired :
+  forall Δ σ d σ__f sitpn Ec τ s s' σ' mm γ id__t σ'__t,
+
+    (* sitpn translates into d. *)
+    sitpn_to_hvhdl sitpn mm = Success d ->
+
+    (* Similar starting states *)
+    s ∼ σ ->
+
+    (* Falling edge from s to s' *)
+    SitpnStateTransition Ec τ s s' falling_edge ->
+
+    (* Falling edge from σ to σf *)
+    vfalling Δ σ (get_behavior d) σ__f ->
+
+    (* Stabilize from σf to σ' *)
+    stabilize Δ σ__f (get_behavior d) σ' ->
+
+    (* Conclusion *)
+    forall t,
+      (** Component idt implements transition t *)
+      γ t = id__t ->
+
+      (* σ't is the state of component idt at design's state σ'. *)
+      MapsTo id__t σ'__t (compstore σ') ->
+
+      (* Conclusion *)
+      @Fired sitpn s' t ->
+      MapsTo Transition.fired (Vbool true) (sigstore σ'__t).
+Proof.
+  intros Δ σ d σ__f.
+  inversion 5.
+  - admit.
+  -
+Admitted.  
