common/StateAndErrorMonad.v
@@ -1,0 +1,50 @@
+(** * State and Error Monad *)
+
+Require Import String.
+
+Section StateAndErrMonad.
+
+  (* A state type *)
+  
+  Variable state : Set.
+
+  (* The value returned by a state-and-error monad can either
+     be an error with a message or a couple state-value.
+   *)
+  
+  Inductive Res (A: Type) (s : state) : Type :=
+  | Error: string -> Res A s
+  | OK: A -> state -> Res A s.
+
+  Arguments OK {A s}.
+  Arguments Error {A s}.
+  
+  Definition Mon (A : Type) : Type := forall s : state, Res A s.
+
+  Definition Ret {A : Type} : A -> Mon A := fun x s => OK x s.
+  Definition Err {A: Type} (msg: string) : Mon A := fun (s: state) => Error msg.
+
+  Definition Bind {A B : Type} : Mon A -> (A -> Mon B) -> Mon B :=
+    fun c1 c2 s1 =>
+      match c1 s1 with
+      | Error msg => Error msg
+      | OK x s2 =>
+        match c2 x s2 with
+        | Error msg => Error msg
+        | OK y s3 => OK y s3
+        end
+      end.
+  Definition Get : Mon state := fun s => OK s s.
+  Definition Put : state -> Mon unit := fun s _ => OK tt s.
+
+End StateAndErrMonad.
+
+Arguments Mon {state}.
+Arguments Err {state A}.
+Arguments Ret {state A}.
+Arguments Bind {state A B}.
+Arguments Get {state}.
+Arguments Put {state}.
+
+Notation "'do' X <- A ; B" := (Bind A (fun X => B))
+                                (at level 200, X ident, A at level 100, B at level 200).
