sitpn/dp/GenerateInfos.v
@@ -8,18 +8,25 @@ Require Import ListsDep.
 Require Import InfosTypes.
 Require Import GlobalTypes.
 Require Import String.
-  
+Require Import StateAndErrorMonad.
+
 Local Open Scope string_scope.
 
 Import ErrMonadNotations.
 
-(** ** Informations about places. *)
-
-Section PlaceInfos.
+Section GenSitpnInfos.
 
   Variable sitpn : Sitpn.
 
-  (** Returns a couple of lists [(i, o)] where [i] is the list of
+  (* The instantiated state type is [SitpnInfo sitpn] *)
+
+  Definition GenInfosMon := @Mon (SitpnInfo sitpn).
+
+  (** ** Informations about places. *)
+
+  Section PlaceInfos.
+    
+    (** Returns a couple of lists [(i, o)] where [i] is the list of
       input transitions of [p], and [o] is the list of output
       transitions of [p].
 
@@ -27,28 +34,29 @@ Section PlaceInfos.
       [i], and [i] has no duplicate, and all output transitions of [p]
       are in [o] and [o] has no duplicate.  *)
 
-  Definition get_neighbors_of_p (p : P sitpn) : optionE (list (T sitpn) * list (T sitpn)) :=
-    (* Adds the transition t to the list of input or output
+    Definition get_neighbors_of_p (p : P sitpn) : GenInfosMon (list (T sitpn) * list (T sitpn)) :=
+      
+      (* Adds the transition t to the list of input or output
        transitions of p. *)
-    let get_neighbor_of_p :=
-        (fun (tin_tout : (list (T sitpn) * list (T sitpn))) t =>
-           let (tin, tout) := tin_tout in
-           match post t p, pre p t with
-           | Some _, Some (_, _) => ((tin ++ [t])%list, (tout ++ [t])%list)
-           | Some _, None => ((tin ++ [t])%list, tout)
-           | None, Some (_, _) => (tin, (tout ++ [t])%list)
-           | None, None => tin_tout
-           end) in
+      let get_neighbor_of_p :=
+          (fun (tin_tout : (list (T sitpn) * list (T sitpn))) t =>
+             let (tin, tout) := tin_tout in
+             match post t p, pre p t with
+             | Some _, Some (_, _) => ((tin ++ [t])%list, (tout ++ [t])%list)
+             | Some _, None => ((tin ++ [t])%list, tout)
+             | None, Some (_, _) => (tin, (tout ++ [t])%list)
+             | None, None => tin_tout
+             end) in
 
-    (* Iterates over the list of transitions, and builds the couple of
+      (* Iterates over the list of transitions, and builds the couple of
        lists (tinputs, touputs) of p along the way by applying
        function is_neighbor_of_p.  *)
-    match tfold_left get_neighbor_of_p (T2List sitpn) (nil, nil) nat_to_T with
-    | (nil, nil) => Err ("Place " ++ $$p ++ " is an isolated place.")
-    | tin_tout => [| tin_tout |]
-    end.
+      match tfold_left get_neighbor_of_p (T2List sitpn) (nil, nil) nat_to_T with
+      | (nil, nil) => Err ("Place " ++ $$p ++ " is an isolated place.")
+      | tin_tout => Ret tin_tout 
+      end.
 
-  (** Injects transition [t] in the list [stranss] depending on the
+    (** Injects transition [t] in the list [stranss] depending on the
       level of priority of [t] compared to the elements of the list
       [stranss].
     
@@ -62,67 +70,68 @@ Section PlaceInfos.
       Correct iff the returned list has no duplicate and its elements
       are ordered by decreasing level of priority. *)
 
-  Fixpoint inject_t (t : T sitpn) (stranss : list (T sitpn)) {struct stranss} :
-    optionE (list (T sitpn)) :=
-    match stranss with
-    (* If the list of priority-ordered transitions is empty, then
+    Fixpoint inject_t (t : T sitpn) (stranss : list (T sitpn)) {struct stranss} :
+      GenInfosMon (list (T sitpn)) :=
+      match stranss with
+      (* If the list of priority-ordered transitions is empty, then
        returns a singleton list where t is the element with the highest
        priority. *)
-    | [] => [| [t] |]
+      | [] => Ret [t]
 
-    (* If there is a head element, compares the head element with t
+      (* If there is a head element, compares the head element with t
      priority-wise. *)
-    | x :: tl =>
+      | x :: tl =>
 
-      (* If t and x are the same, then t has already been injected in
+        (* If t and x are the same, then t has already been injected in
        stranss, then stranss is returned. That case does not happen
        given a proof of [~In t stranss], that is, t is not among 
        the first elements of stranss.
 
        Otherwise, checks if t has a higher firing priority than x. *)
-      if Teqdec t x then [| stranss |]
-      else
-        (* If t is the element with the highest priority, then puts it
+        if Teqdec t x then Ret stranss
+        else
+          (* If t is the element with the highest priority, then puts it
            as the head element of stranss, and returns the list.
          
          Otherwise, checks if x has a higher priority than t.  *)
-        if t >~ x then [| t :: stranss |]
-        else
-          (* If x has a higher priority than t, then tries to inject t
-           in the list's tail.  *)
-          if x >~ t then
-            (* Error case: found a transition that is not comparable
-               with t in the list's tail.  *)
-            stranss' <- inject_t t tl; [| x :: stranss' |]
+          if t >~ x then Ret (t :: stranss)
           else
-            (* Error case: t >~ x and x >~ t evaluate to false. *)
-            Err ("Transitions " ++ $$t ++ " and " ++ $$x ++ " are not comparable with the priority relation.")
-    end.
+            (* If x has a higher priority than t, then tries to inject t
+           in the list's tail.  *)
+            if x >~ t then
+              (* Error case: found a transition that is not comparable
+               with t in the list's tail.  *)
+              do stranss' <- inject_t t tl; Ret (x :: stranss')
+            else
+              (* Error case: t >~ x and x >~ t evaluate to false. *)
+              Err ("Transitions " ++ $$t ++ " and " ++ $$x ++ " are not comparable with the priority relation.")
+      end.
 
-  (** Injects all transitions of the [transs] list in the list [stranss]
+    (** Injects all transitions of the [transs] list in the list [stranss]
       that contains transitions sorted by level of firing priority.  *)
 
-  Fixpoint sort_by_priority_aux
-           (transs : list (T sitpn))
-           (stranss : list (T sitpn)) {struct transs} :
-    optionE (list (T sitpn)) :=
-    match transs with
-    | [] => [| stranss |]
-    | t :: tl =>
-      stranss' <- inject_t t stranss; sort_by_priority_aux tl stranss'
-    end.
+    Fixpoint sort_by_priority_aux
+             (transs : list (T sitpn))
+             (stranss : list (T sitpn)) {struct transs} :
+      GenInfosMon (list (T sitpn)) :=
+      match transs with
+      | [] => Ret stranss
+      | t :: tl =>
+        do stranss' <- inject_t t stranss;
+        sort_by_priority_aux tl stranss'
+      end.
 
-  (** Takes a list of transitions [transs], and returns a new list of
+    (** Takes a list of transitions [transs], and returns a new list of
       transitions where the elements are ordered by level of firing
       priority.
 
       Raises an error if no strict total ordering can be established
       in relation to the priority order.  *)
 
-  Definition sort_by_priority (transs : list (T sitpn)) :
-    optionE (list (T sitpn)) := sort_by_priority_aux transs [].
+    Definition sort_by_priority (transs : list (T sitpn)) :
+      GenInfosMon (list (T sitpn)) := sort_by_priority_aux transs [].
 
-  (** Returns a PlaceInfo structure containing the information related
+    (** Returns a PlaceInfo structure containing the information related
       to place [p], a place of [sitpn].
 
       Error cases :
@@ -132,38 +141,38 @@ Section PlaceInfos.
 
       - the priority relation is not a strict total order over the
         output transitions of t. 
-   *)
-
-  Definition get_p_info (p : P sitpn) : optionE (P sitpn * PlaceInfo sitpn) :=
-
-    (* Gets the input and output transitions list of place p. 
-       Error: p is an isolated place.
      *)
-    tin_tout <- get_neighbors_of_p p;
-    (* Sorts the output transitions of p by decreasing level of firing
+
+    Definition add_pinfo (p : P sitpn) : GenInfosMon unit :=
+
+      (* Gets the input and output transitions list of place p. 
+       Error: p is an isolated place.
+       *)
+      do tin_tout <- get_neighbors_of_p p;
+      (* Sorts the output transitions of p by decreasing level of firing
        priority. 
        Error: the priority relation is not a strict total order
        over the output transitions of p.
-     *)
-    let '(tin, tout) := tin_tout in
-    stout <- sort_by_priority tout;
-    [| (p, MkPlaceInfo _ tin stout) |].
-  
-  (** Computes information for all p ∈ P, and returns the list of
+       *)
+      let '(tin, tout) := tin_tout in
+      do stout <- sort_by_priority tout;
+      do sitpninfo <- Get;
+      Put (set_pinfo (p, MkPlaceInfo _ tin stout) sitpninfo).
+    
+    (** Computes information for all p ∈ P, and returns the list of
       couples implementing function P → PlaceInfo. *)
-  
-  Definition generate_place_infos : optionE (list (P sitpn * PlaceInfo sitpn)) :=    
-    topte_map get_p_info (P2List sitpn) nat_to_P.
-  
-End PlaceInfos.
+    
+    Definition generate_place_infos : GenInfosMon unit :=
+      do s <- Get;
+      tfold_left (fun s p => add_pinfo p) (P2List sitpn) (Put s) nat_to_P.
+    
+  End PlaceInfos.
 
-(** ** Informations about transitions. *)
+  (** ** Informations about transitions. *)
 
-Section TransitionInfos.
+  Section TransitionInfos.
 
-  Variable sitpn : Sitpn.
-  
-  (** Returns the list of input places of transition [t].
+    (** Returns the list of input places of transition [t].
 
     Correctness: Correct iff all input places of [p] are in the
     returned list, and the returned has no duplicates.
@@ -172,39 +181,49 @@ Section TransitionInfos.
     doesn't mean that [t] is an isolated transition; however [t] is a
     "source" transition (without input).
     
-   *)
+     *)
 
-  Definition get_inputs_of_t (t : T sitpn) : list (P sitpn) :=    
-    (* Tests if a place is an input of t. *)
-    let is_input_of_t := (fun p => if (pre p t) then true else false) in
-    tfilter is_input_of_t (P2List sitpn) nat_to_P.
+    Definition get_inputs_of_t (t : T sitpn) : GenInfosMon (list (P sitpn)) :=    
+      (* Tests if a place is an input of t. *)
+      let is_input_of_t := (fun p => if (pre p t) then true else false) in
+      Ret (tfilter is_input_of_t (P2List sitpn) nat_to_P).
 
-  (** Returns the list of conditions associated to transition [t].
+    (** Returns the list of conditions associated to transition [t].
     
     Correctness: Correct iff all conditions associated to [t] are in the
     returned list, and the returned has no duplicates.  *)
 
-  Definition get_conds_of_t (t : T sitpn) : list (C sitpn) :=
-    (* Tests if a condition is associated to t. *)
-    let is_cond_of_t := (fun c => (match has_C t c with one | mone => true | zero => false end)) in
-    tfilter is_cond_of_t (C2List sitpn) nat_to_C.
-  
-  (** Computes the information about transition t, and returns
+    Definition get_conds_of_t (t : T sitpn) : GenInfosMon (list (C sitpn)) :=
+      (* Tests if a condition is associated to t. *)
+      let is_cond_of_t := (fun c => (match has_C t c with one | mone => true | zero => false end)) in
+      Ret (tfilter is_cond_of_t (C2List sitpn) nat_to_C).
+    
+    (** Computes the information about transition t, and returns
       a couple [(t, info)].
-   *)
+     *)
 
-  Definition get_t_info (t : T sitpn) : (T sitpn * TransInfo sitpn) :=
-    (t, MkTransInfo _ (get_inputs_of_t t) (get_conds_of_t t)).
+    Definition add_tinfo (t : T sitpn) : GenInfosMon unit :=
+      do inputs_of_t <- get_inputs_of_t t;
+      do conds_of_t <- get_conds_of_t t;
+      do sitpninfo <- Get;
+      Put (set_tinfo (t, MkTransInfo _ inputs_of_t conds_of_t) sitpninfo).
 
-  (** Maps the function [get_t_info] to the list of transitions of [sitpn],
+    (** Maps the function [get_t_info] to the list of transitions of [sitpn],
       and returns the resulting list of couples [(t, info)]. *)
 
-  Definition generate_trans_infos : list (T sitpn * TransInfo sitpn) :=
-    tmap get_t_info (T2List sitpn) nat_to_T.
-  
-End TransitionInfos.
+    Definition generate_trans_infos : GenInfosMon unit :=
+      do s <- Get;
+      tfold_left (fun s t => get_t_info t) (T2List sitpn) nat_to_T.
+    
+  End TransitionInfos.
 
-Arguments generate_trans_infos {sitpn}.
+  Arguments generate_trans_infos {sitpn}.
+  
+  
+End GenSitpnInfos.
+
+
+
 
 (** ** Informations about conditions, actions and functions. *)
 
