sitpn2hvhdl/Sitpn2HVhdlTypes.v
@@ -1,8 +1,11 @@
 (** * Sitpn2HVhdhl intermediary types.  *)
 
+Require Import Coqlib.
+Require Import String.
 Require Import HVhdlTypes.
 Require Import AbstractSyntax.
 Require Import dp.Sitpn.
+Require Import StateAndErrorMonad.
 
 (** ** Types used in the Sitpn2HVhdl transformation. *)
 
@@ -50,10 +53,38 @@ Definition FunMap sitpn := list (F sitpn * list expr).
 
 Definition Architecture sitpn := (list adecl * PlaceMap sitpn * TransMap sitpn * FunMap sitpn * ActionMap sitpn)%type.
 
+(** **  Source to target binder *)
+
+(** Maps the elements of an SITPN to their signal or component
+    identifiers on the VHDL side. *)
+
+Record Sitpn2HVhdlMap sitpn : Type :=
+  BuildMap {
+      p2pcomp : list (P sitpn * ident);
+      t2pcomp : list (T sitpn * ident);
+      a2out   : list (A sitpn * ident);
+      f2out   : list (F sitpn * ident);
+      c2in    : list (C sitpn * ident);
+    }.
+
 (** ** Compile-time state *)
 
 Record Sitpn2HVhdlState sitpn : Type :=
   BuildState {
+
+      (* Next id *)
+      nextid : ident;
+      
+      (* Architecture in intermediary format *)
       arch : Architecture sitpn;
 
+      (* Source-to-target binder *)
+      γ : Sitpn2HVhdlMap sitpn;
+
+      (* Architecture body in VHDL abstract syntax *)
+      behavior : cs;
     }.
+
+(** *** Operations on Compile-time State *)
+
+
